WIP: fixing wiring again

nondeterministic_dataflow/Timely_Operators.thy
@@ -280,6 +280,12 @@ datatype ('id, 'p, 's, 'd) dataflow_tree =
    | Comp "'id \<times> 'p \<Rightarrow> ('id \<times> 'p) option" "('id, 'p, 's, 'd) dataflow_tree" "('id, 'p, 's, 'd) dataflow_tree"
 
 
+definition tscomp_op ::
+  "('ip option, 'op1 option, 'd + 's) op \<Rightarrow>
+   ('op1 option, 'op option, 'd + 's) op \<Rightarrow>
+   ('ip option, 'op option, 'd + 's) op" (infixl "\<bullet>\<^sub>t" 65) where
+  "tscomp_op op1 op2 = map_op (case_sum id (\<lambda> _. None)) (case_sum (\<lambda> _. None) id) (comp_op (case_option None (Some o Some)) (\<lambda>_. []) op1 op2)"
+
 fun compile_dataflow_tree_aux :: "'id :: {minus, plus, one, ord} \<Rightarrow> ('id, 'p, 's, 'd) dataflow_tree \<Rightarrow>
     'id \<times> (('id, 'p) location \<Rightarrow> ('id, 'p) location \<Rightarrow> nat antichain) \<times> ('id + 'id \<times> 'p, 'id + 'id \<times> 'p, 's + 'd) op" where
   "compile_dataflow_tree_aux n (Comp wire dt1 dt2) = (
@@ -287,11 +293,12 @@ fun compile_dataflow_tree_aux :: "'id :: {minus, plus, one, ord} \<Rightarrow> (
     let (n'', summary2, op2) = compile_dataflow_tree_aux n' dt2 in
     (n'', \<lambda> l1 l2. 
      if node l1 \<ge> n \<and> node l1 < n' \<and> node l2 \<ge> n' \<and> is_Src (port l1) \<and> is_Trg (port l2)
-     then (case wire (node l1 - n, idp (port l1)) of 
+     then (case wire (node l1, idp (port l1)) of 
              None \<Rightarrow> frontier {#}\<^sub>z 
-           | Some (offset, q) \<Rightarrow> (if node l2 = n' + offset \<and> q = idp (port l2) then frontier (abs_zmultiset (mset [0], {#})) else frontier {#}\<^sub>z )) 
+           | Some (offset, q) \<Rightarrow> (if node l2 = offset \<and> q = idp (port l2) then frontier (abs_zmultiset (mset [0], {#})) else frontier {#}\<^sub>z )) 
      else summary1 l1 l2 + summary2 l1 l2,
-     map_op (case_sum id id) (case_sum id id) (comp_op (case_sum (Some o Inl) ((case_option None (Some o Inr)) o wire)) (\<lambda> _. []) op1 op2))
+     map_op (case_sum id id) (case_sum id id)
+     (comp_op (case_sum (\<lambda> _. None) ((case_option None (Some o Inr)) o wire)) (\<lambda> _. []) op1 op2))
    )"
 | "compile_dataflow_tree_aux n (Logic op) = (n + 1,
     (\<lambda> l1 l2. 
@@ -301,29 +308,10 @@ fun compile_dataflow_tree_aux :: "'id :: {minus, plus, one, ord} \<Rightarrow> (
     map_op (case_option (Inl n) (\<lambda> p. Inr (n, p))) (case_option (Inl n) (\<lambda> p. Inr (n, p))) op)"
 
 value  "(fst o snd) (compile_dataflow_tree_aux (0 :: 4)
-       (Comp Some
+       (Comp [ (1, 0) \<mapsto> (3, 0) ]
          (Comp (\<lambda> l. None) (Logic \<oslash>) (Logic \<oslash>))
          (Comp (\<lambda> l. None) (Logic \<oslash>) (Logic \<oslash>))))
       (Loc 1 (Src 1)) (Loc 3 (Trg (1 :: 1)))"
-
-term  "(snd o snd) (compile_dataflow_tree_aux (0 :: 4)
-       (Comp Some
-         (Comp (\<lambda> l. None) (Logic (\<I> :: (1 option, 1 option, unit + nat) op)) (Logic \<I>))
-         (Comp (\<lambda> l. None) (Logic \<I>) (Logic \<I>))))"
-
-(* 
-value "(fst o snd) (compile_dataflow_tree_aux (0 :: 4)
-       (Comp Some
-         (Comp (\<lambda> l. None) (Logic (\<lambda> _. \<oslash>)) (Logic (\<lambda> _. \<oslash>)))
-         (Comp (\<lambda> l. None) (Logic (\<lambda> _. \<oslash>)) (Logic (\<lambda> _. \<oslash>)))))
-      (Loc 1 (Trg 1)) (Loc 1 (Src (1 :: 1)))"
-
-
-value "(fst o snd) (compile_dataflow_tree_aux (0 :: 5)
-       (Comp [(1, 1) \<mapsto> (0, 1), (2, 1) \<mapsto> (1, 1)]
-         (Comp (\<lambda> l. None) (Comp Some (Logic (\<lambda> _. \<oslash>)) (Logic (\<lambda> _. \<oslash>))) (Logic (\<lambda> _. \<oslash>)))
-         (Comp (\<lambda> l. None) (Logic (\<lambda> _. \<oslash>)) (Logic (\<lambda> _. \<oslash>)))))
-      (Loc 2 (Src (1 :: 1))) (Loc 4 (Trg (1 :: 1)))" *)
 
 definition "compile_dataflow_tree df = (
   let (_, s, op) = compile_dataflow_tree_aux 0 df in
@@ -333,18 +321,14 @@ definition "compile_dataflow_tree df = (
   then (s, op)
   else Code.abort (STR ''Control plane could not be build'') (\<lambda> _. (\<lambda> _ _. frontier {#}\<^sub>z, \<oslash>)))"
 
-abbreviation "df_ex1 \<equiv> (Comp Some
+abbreviation "df_ex1 \<equiv> (Comp [ (1, 0) \<mapsto> (3, 0) ]
          (Comp (\<lambda> l. None) (Logic \<oslash>) (Logic \<oslash>))
          (Comp (\<lambda> l. None) (Logic \<oslash>) (Logic \<oslash>))) :: (4, 4, unit, nat) dataflow_tree"
-
-abbreviation "df_ex2 \<equiv> (Comp Some (Logic \<oslash>) (Logic \<oslash>)) :: (2, 2, unit, nat) dataflow_tree"
-
 
 value "fst (compile_dataflow_tree
        df_ex1)
        (Loc 1 (Src (0 :: 4))) (Loc 3 (Trg 0))"
 
-term "compile_dataflow_tree"
 
 lemma compile_dataflow_tree_aux_same_loc:
   "(n'', summar, op) = compile_dataflow_tree_aux n df \<Longrightarrow>
@@ -417,10 +401,6 @@ lemma empty_graph_no_zero_cyc:
     done
   done
 
-lemma no_self_loop_checker_is_graph_checker:
-  "no_self_loop_checker = graph_checker"
-  sorry
-
 lemma enum_dataflow_topology_compile_dataflow[simp]:
   "enum_dataflow_topology (fst (compile_dataflow_tree df)) (+)"
   apply standard
@@ -478,8 +458,6 @@ declare dataflow_topology_from_tree.take_step.simps[of _ "((<) :: nat \<Rightarr
 abbreviation empty_conf where
   "empty_conf \<equiv> \<lparr>c_work = (\<lambda> _.  {# 0 #}\<^sub>z), c_pts = (\<lambda> _.  {#}\<^sub>z), c_imp = (\<lambda> _. {#}\<^sub>z)\<rparr>"
 
-value "propagate_all_locale (fst (compile_dataflow_tree df_ex2)) df_ex2 empty_conf"
-
 definition "propagate_all summary c0 = (while_option (Not o (worklist_is_empty summary))
                                         (take_step summary PR) c0)"
 
@@ -493,8 +471,6 @@ lemma take_step_fast_code[simp]:
 lemma propagate_all_locale_eq_propagate_all:
   "propagate_all_locale (fst (compile_dataflow_tree df)) df c = propagate_all (fst (compile_dataflow_tree df)) c"
   unfolding propagate_all_locale_def Let_def propagate_all_def by (auto split: prod.splits)
-
-value "propagate_all (fst (compile_dataflow_tree df_ex2)) empty_conf"
 
 fun print_2 where
   "print_2 n = (if n = 0 then STR ''0'' else STR ''1'')"
@@ -514,12 +490,13 @@ abbreviation "trace \<equiv> (if DEBUG then Debug.tracing else (\<lambda> x y. y
 (* Inspired by timely/src/progress/subgraph.rs:453 *)
 (* First migrate all change batches to the worklist, then call propagate_all_locale *)
  fun propagate_pointstamps where
-  "propagate_pointstamps summary conf [] = propagate_all summary conf"
+  "propagate_pointstamps summary conf [] = trace (STR ''Propagating all'') propagate_all summary conf"
 | "propagate_pointstamps summary conf ((l, t, m) # cbs) =
    propagate_pointstamps summary (trace (STR ''CM ==> '' + show_loc l + STR '', t: '' + show_nat t + STR '', m: '' + print_int m) (take_step summary (CM l t m)) conf) cbs"
 
+
 abbreviation "init_subgraph summary \<equiv>
-  \<lparr> pt_tr = the (propagate_pointstamps summary empty_conf [(Loc 0 (Src 1), 0, 1)]),
+  trace (STR ''Initializing subgraph'') \<lparr> pt_tr = the (propagate_pointstamps summary empty_conf (concat (map (\<lambda> nid. map (\<lambda> p. (Loc nid (Src p), 0, 1)) enum_class.enum) enum_class.enum))),
    lo_pt = [],
    edges = (\<lambda> l1. [l2 \<leftarrow> enum_location_inst.enum_location. \<not> is_empty_antichain (summary l1 l2) ]),
    summ = summary \<rparr>"
@@ -538,45 +515,46 @@ definition extract_progress where
     map (\<lambda> (p, t, m). (Loc nid (Src p), t, m)) (inte st) @
     concat (map (\<lambda> (p, t, m). map (\<lambda> l. (l, t, m)) (edg (Loc nid (Src p)))) (prod st))"
 
-lift_definition Max_antichain :: "nat antichain \<Rightarrow> nat" is "\<lambda> x. if Set.is_empty x then 0 else Max x" .
+lift_definition Max_antichain :: "nat antichain \<Rightarrow> nat" is "\<lambda> x. if Set.is_empty x then 42 else Max x" .
 
-abbreviation "print_frontier x \<equiv> trace (show_nat (Max_antichain x))" 
+abbreviation "print_frontier x \<equiv> trace ((STR ''Frontier: '') + show_nat (Max_antichain x))" 
 
 (* Inspired by timely/src/dataflow/operators/capability.rs:62 *)
 datatype ('p, 't) capability = Cap (time: 't) (out: 'p)
 
 abbreviation "frontier_updating b \<equiv> cfilter (\<lambda> op. case op of Read (Inl _) f \<Rightarrow> b | _ \<Rightarrow> True)"
 
+(* TODO: nid must have a concrete type *)
 corec dataflow_op where
-  "dataflow_op b sg op = Choice (cimage (\<lambda> op. case op of 
-     Read (Inl (nid :: 2))  f \<Rightarrow> let imp_fron = (\<lambda> p. c_imp (pt_tr sg) (Loc nid (Trg p))) in Silent (dataflow_op False sg (f (Inr (Inr imp_fron))))
-   | Read (Inr (nid, p)) f \<Rightarrow> Read p (\<lambda> x. dataflow_op b sg (f (Inl x)))
-   | Write op' (Inl nid) (Inr (Inl st)) \<Rightarrow> (case propagate_pointstamps (summ sg) (pt_tr sg) (lo_pt sg @ extract_progress nid (edges sg) st) of
-                                              Some conf' \<Rightarrow> Silent (dataflow_op True (sg\<lparr> pt_tr := conf', lo_pt := [] \<rparr>) op'))
-   | Write op' (Inr (nid, p)) (Inl x) \<Rightarrow> Write (dataflow_op b sg op') p x
-   | Silent op' \<Rightarrow> Silent (dataflow_op b sg op')) (frontier_updating b (choices op)))"
+  "dataflow_op sg op = Choice (cimage (\<lambda> op. case op of 
+     Read (Inl (nid :: 2)) f \<Rightarrow> let imp_fron = (\<lambda> p. c_imp (pt_tr sg) (Loc nid (Trg p))) in Silent (dataflow_op sg (f (Inl (Inr imp_fron))))
+   | Read (Inr (nid, p)) f \<Rightarrow> Read (nid, p) (\<lambda> x. dataflow_op sg (f (Inr x)))
+   | Write op' (Inl nid) (Inl (Inl st)) \<Rightarrow> (case propagate_pointstamps (summ sg) (pt_tr sg) (lo_pt sg @ extract_progress nid (edges sg) st) of
+                                              Some conf' \<Rightarrow> Silent (dataflow_op (sg\<lparr> pt_tr := conf', lo_pt := [] \<rparr>) op'))
+   | Write op' (Inr (nid, p)) (Inr x) \<Rightarrow> Write (dataflow_op sg op') (nid, p) x
+   | Silent op' \<Rightarrow> Silent (dataflow_op sg op')) (choices op))"
 
 
 definition "compile_dataflow dt = (let (summary, op) = compile_dataflow_tree dt in
                                     let sg = init_subgraph summary in
-                                    dataflow_op True sg op)"
+                                    dataflow_op sg op)"
 
 (* Should this be non-deterministic? (e.g. non-deterministically send events and capabilities updates) *)
 (* Inspired by timely/src/dataflow/channels/pushers/counter.rs:25 and timely/src/dataflow/channels/mod.rs:49 *)
 (* writes maybe could support multiple different ports, then this one also would *)
 abbreviation "push op p batch \<equiv> 
-  writes (Write op None (Inr (Inl \<lparr> cons = [], inte = [], prod = map (\<lambda> (x, c). (p, time c, 1)) batch \<rparr>))) (Some p) (map (\<lambda> (x, c). Inl (x, time c)) batch)"
+  writes (Write op (trace (STR ''Pushing data!'') None) (Inl (Inl \<lparr> cons = [], inte = [], prod = map (\<lambda> (x, c). (p, time c, 1)) batch \<rparr>))) (Some p) (map (\<lambda> (x, c). Inr (x, time c)) batch)"
 
 abbreviation "drop_cap c op \<equiv>
-  Write op None (trace (String.implode (''Dropping cap!'')) Inr (Inl \<lparr> cons = [], inte = [(out c, time c, -1)], prod = [] \<rparr>))"
+  Write op None (trace (String.implode (''Dropping cap!'')) Inl (Inl \<lparr> cons = [], inte = [(out c, time c, -1)], prod = [] \<rparr>))"
 
 abbreviation "drop_caps cs op \<equiv>
-  Write op None (trace (String.implode (''Dropping caps!'')) Inr (Inl \<lparr> cons = [], inte = map (\<lambda> c. (out c, time c, -1)) cs, prod = [] \<rparr>))"
+  Write op None (trace (String.implode (''Dropping caps!'')) Inl (Inl \<lparr> cons = [], inte = map (\<lambda> c. (out c, time c, -1)) cs, prod = [] \<rparr>))"
 
 abbreviation "delayed_cap c t \<equiv>
   (Cap (time c + abs t) (out c),
   \<lambda> op. Write op None 
-     (Inr (Inl \<lparr> cons = [],
+     (Inl (Inl \<lparr> cons = [],
             inte = [(out c, time c, -1), (out c, time c + abs t, 1)],
             prod = [] \<rparr>)))"
 
@@ -588,23 +566,16 @@ abbreviation "delayed_cap c t \<equiv>
 corec input_op where
   "input_op c inps = (case inps of
     LNil \<Rightarrow> drop_cap c \<oslash>
-  | LCons xs lxs \<Rightarrow> push (Write (input_op (Cap (time c + 1) (out c)) lxs) None 
-     (trace (STR ''Delaying capability!'') Inr (Inl \<lparr> cons = [],
-            inte = [(out c, time c, -1), (out c, time c + 1, 1)],
-            prod = []\<rparr>))) 1 (map (\<lambda> x. (x, c)) xs))"
+  | LCons xs lxs \<Rightarrow>
+     push 
+     (Write (input_op (Cap (time c + 1) (out c)) lxs) (trace (STR ''Delaying cap'') None) (Inl (Inl \<lparr> cons = [], nte = [(out c, time c, -1), (out c, time c + 1, 1)], prod = []\<rparr>)))
+      1 (map (\<lambda> x. (x, c)) xs))"
 
 abbreviation "ex1 \<equiv> Logic (input_op (Cap 0 (1 :: 1)) (LCons [Suc 0] LNil))"
 
-value [GHC] "eval 2 (compile_dataflow ex1)"
+value [GHC] "eval 20 (compile_dataflow ex1)"
 
-abbreviation "ex2 \<equiv> Comp [ (0, 0) \<mapsto> (1, 0) ] ex1 (Logic \<I>)"
-
-value [GHC] "cfilter ((\<noteq>) []) (eval 6 (compile_dataflow ex2))"
-
-
-end
-
-term "( (input_op (Cap (0 :: nat) (0 :: 2)) (LCons [Suc 0, 2, 3, 9] (LCons [8, 1, 0] LNil))))"
+term "compile_dataflow ex1"
 
 (* value [GHC] "eval 17 (dataflow_op True init_subgraph (input_op (Cap (0 :: nat) 0) (LCons [Suc 0, 2, 3, 9] (LCons [8, 1, 0] LNil))))"
 value [GHC] "eval 5 (dataflow_op True init_subgraph (input_op (Cap (0 :: nat) 0) (LCons [Suc 0] (LNil))))"
@@ -612,9 +583,9 @@ value [GHC] "eval 5 (dataflow_op True init_subgraph (input_op (Cap (0 :: nat) 0)
 abbreviation "maxs ft buf \<equiv> [(n, c) \<leftarrow> buf. ft (time c) \<and> n = Max (set (map fst ((filter (\<lambda> (n', c'). time c = time c') buf))))]"
 
 (* The minted capability must depend on the internal wiring *)
-abbreviation "pull nid i f \<equiv> (Read (Some i) 
+abbreviation "pull i f \<equiv> (Read ((trace (STR ''Reading data'') Some) i)
   (\<lambda> x. case x of
-    (Inl (d, t)) \<Rightarrow> Write (f (d, Cap t 0)) None (Inr (Inl \<lparr>  cons = [(nid, i, t, 1)], inte = [(nid, i, t, 1)], prod = [] \<rparr>))))"
+    (Inr (d, t)) \<Rightarrow> Write (f (d, Cap t 0)) None (Inl (Inl \<lparr>  cons = [(i, t, 1)], inte = [(i, t, 1)], prod = [] \<rparr>))))"
 
 abbreviation
   "less_than_frontier ft t \<equiv> (\<not> is_empty_antichain (filter_antichain (\<lambda> f. t < f) ft))"
@@ -623,19 +594,23 @@ term choice2
 
 declare [[unify_search_bound = 100]]
 
-corec max_op' :: "(nat \<times> (2, nat) capability) buf \<Rightarrow> (2 option, 2 option, nat \<times> nat + (2, nat) shared_state + (2 location \<Rightarrow> nat zmultiset)) op" where
+corec max_op' where
   "max_op' buf = choice2
-   (Read None (\<lambda> st.
-    let impf = projr (projr st) in
-    let ft = frontier (impf (Loc 1 (Trg 0))) in
-    if is_empty_antichain ft 
-    then \<oslash> 
+   (Read (trace (STR ''Reading frontier'') None) (\<lambda> st.
+    let impf = projr (projl st) in
+    let ft = frontier (impf 0) in
+    if print_frontier ft  is_empty_antichain ft 
+    then trace (STR ''Empty frontier'') \<oslash> 
     else 
-    let result = (maxs (less_than_frontier ft) buf) in
-    push 1 (drop_caps 1 (map snd result) (max_op' [(n, c) \<leftarrow> buf. \<not> less_than_frontier ft (time c)])) 0 result))
-   (pull (1 :: 2) (0 :: 2) (\<lambda> x. max_op' (buf @ [x])))"
+    let result = trace (STR ''Non empty frontier'') (maxs (less_than_frontier ft) buf) in
+    push (drop_caps (map snd result) (max_op' [(n, c) \<leftarrow> buf. \<not> less_than_frontier ft (time c)])) 0 result))
+   (pull (0 :: 1) (\<lambda> x. max_op' (buf @ [x])))"
 
 abbreviation "max_op \<equiv> max_op' []"
+
+value [GHC] "approx_in 60 [VOut (1, 0) (1, 0)] (compile_dataflow (Comp [ (0, 0) \<mapsto> (1, 0) ] ex1 (Logic max_op)))"
+
+term "show_list (show_nat)"
 
 (* corec max_op :: "(nat \<times> (2, nat) capability) buf \<Rightarrow> (2 option, 2 option, nat \<times> nat + (2, nat) shared_state + (2 location \<Rightarrow> nat zmultiset)) op" where
   "max_op buf = Read None (\<lambda> st. pull (1 :: 2) (0 :: 2) (case_option
@@ -647,17 +622,6 @@ abbreviation "max_op \<equiv> max_op' []"
 (* value [GHC] "approx_in 36 [VOut 0 (9, 0), VOut 0 (5, 1)] (dataflow_op True init_subgraph ((input_op (Cap (0 :: nat) (0 :: 2)) (LCons [9, 3] (LCons [5] LNil))) \<bullet>\<^sub>t max_op))"
  *)
 
-
-
-(*
-instantiation bit0 :: (finite) defaults begin
-definition defaults_bit0 :: "'a bit0 set" where "defaults_bit0 = {}"
-instance ..
-end
-instantiation bit1 :: (finite) defaults begin
-definition defaults_bit1 :: "'a bit1 set" where "defaults_bit1 = {}"
-instance ..
-end *)
 
 
 end
